We know that in order to solve the Einstein Equation for no Energy Momentum Tensor, we must solve for $R_{\mu \nu} = 0$

Setting the above to equal to zero gives us four equations:

$R_{t t} = 0 \Leftrightarrow $ Equation 1: $$ \frac{A''}{2B} - \frac{A'B'}{4B^2} - \frac{(A')^2}{4AB} + \frac{A'}{rB}= 0$$

$R_{r r} = 0 \Leftrightarrow $ Equation 2: $$ \frac{A''}{2A} + \frac{A'B'}{4AB} + \frac{(A')^2}{4A^2} + \frac{B'}{rB} = 0$$

$R_{\theta \theta} = 0 \Leftrightarrow $ Equation 3: $$ \frac{rB}{2B^2} - \frac{rA'}{2AB} + 1 + \frac{1}{B} = 0$$

$R_{\phi \phi} = 0 \Leftrightarrow $ Equation 4: $$ \sin^2(\theta) \left(\frac{rAB'}{2AB^2} - \frac{rBA'}{2AB^2} + 1 - \frac{1}{B} \right) = 0$$

It is easy to see how one might simplify these, but lets skip ahead and combine some of these to get to what we want. (Expressions of $A(r)$ and $B(r)$.) Namely, we will do the following to Equation 1 and Equation 2:

Define a new Equation 5: $$ \left( B \times Equation1 + A \times Equation2 \right) \times (rB)$$